\documentclass{article}
\usepackage{epsfig}
\pagestyle{empty}
\begin{document}
$T$
\pagebreak

$x_0$
\pagebreak

$ \mu_{x_{t-1}\rightarrow x_t}(x)=\mathcal{N}(x_t|s_t,S_t) $
\pagebreak

$ s_t=a_{t-1}\!+\!A_{t-1}(S_{t-1}^{-1}\!+\!R_{t-1})^{-1}(S_{t-1}^{-1}s_{t-1}\!+\!r_{t-1}) $
\pagebreak

$ S_t=Q+B_tH^{-1}B_t^{\!\top\!} + A_{t-1}(S_{t-1}^{-1}+R_{t-1})^{-1}A_{t-1}^{\!\top\!} $
\pagebreak

$ \mu_{x_{t+1}\rightarrow x_t}(x)=\mathcal{N}(x_t|v_t,V_t) $
\pagebreak

$ v_t=-A_{t}^{-1}a_{t}\!\!+\!\!A_{t}^{-1}(V_{t+1}^{-1}\!\!+\!\!R_{t+1})^{-1}(V_{t+1}^{-1}v_{t+1}\!\!+\!\!r_{t+1}) $
\pagebreak

$ V_t=A_{t}^{-1}[Q+B_tH^{-1}B_t^{\!\top\!} + (V_{t+1}^{-1}+R_{t+1})^{-1}]A_{t}^{-{\!\top\!}} $
\pagebreak

$ \mu_{z_t\rightarrow x_t}(x)=\mathcal{N}[x_t|r_t,R_t] $
\pagebreak

$ b_t(X_t)=\mu_{x_{t-1}\rightarrow x_t}(x) \mu_{x_{t+1}\rightarrow x_t}(x) \mu_{z_t\rightarrow x_t}(x) $
\pagebreak

$ b_t(X_t)=\mathcal{N}\left(x_t|(S_t^{-1}+V_t^{-1}+R_t)^{-1}(S_t^{-1}s_t+V_t^{-1}v_t+r_t),S_t^{-1}+V_t^{-1}+R_t \right) $
\pagebreak

$ R, r, \hat{r} $
\pagebreak

$t$
\pagebreak

$x=Ab$
\pagebreak

\end{document}
